\subsection{Opór zastępczy}
\subsubsection{Szeregowe łączenie rezystorów}
\begin{schemat}
\draw
 node[ocirc] (A) at (0,0) {}
 node[ocirc] (B) at (4,0) {}
 (0,0) to[R,l=$R_1$] (2,0) 
 (2,0) to[R,l=$R_2$] (4,0)
;
\end{schemat}

\begin{equation}
R_z=R_1+R_2
\end{equation}

\begin{schemat} 
\draw
 node[ocirc] (A) at (0,0) {}
 node[ocirc] (B) at (8,0) {}
 (0,0) to[R,l=$R_1$] (2,0) 
 (2,0) to[R,l=$R_2$] (4,0)
 (6,0) to[R,l=$R_n$] (8,0)
;
\end{schemat}
\begin{equation}
R_z=R_1+R_2+...+R_n
\end{equation}

\subsubsection{Równoległe łączenie rezystorów}

\begin{schemat} 
\draw
 node[ocirc] (A) at ( 0, 0) {}
 node[ocirc] (B) at ( 4, 0) {}
 ( 0, 0) to[short]     ( 1, 0)
 ( 1, 0) to[short]     ( 1, 1)
 ( 1, 0) to[short]     ( 1,-1)
 ( 1, 1) to[R,l=$R_1$] ( 3, 1) 
 ( 1,-1) to[R,l=$R_2$] ( 3,-1)
 ( 3, 1) to[short]     ( 3, 0)
 ( 3,-1) to[short]     ( 3, 0)
 ( 3, 0) to[short]     ( 4, 0)
;
\end{schemat}

\begin{equation}
R_z=\frac{R_1 \cdot R_2}{R_1+R_2}
\end{equation}

\begin{schemat}
\draw
 node[ocirc] (A) at ( 0, 0) {}
 node[ocirc] (B) at ( 4, 0) {}
 ( 0, 0) to[short]     ( 1, 0)
 ( 1, 0) to[short]     ( 1, 1)
 ( 1, 0) to[short]     ( 1,-0.5)
 ( 1, -1) to[short]     ( 1,-1.5)
 ( 1, 1) to[R,l=$R_1$] ( 3, 1) 
 ( 1, 0) to[R,l=$R_2$] ( 3, 0)
 ( 1, -1.5) to[R,l=$R_n$] ( 3, -1.5)
 ( 3, 1) to[short]     ( 3, 0)
 ( 3,-0.5) to[short]   ( 3, 0)
 ( 3,-1) to[short]   ( 3, -1.5)
 ( 3, 0) to[short]     ( 4, 0)
;
\end{schemat}

\begin{equation}
\frac{1}{R_z}=\frac{1}{R_1} + \frac{1}{R_2} + ... + \frac{1}{R_n}
\end{equation}