\subsection{Przekształcenie trójkat-gwiazda i gwiazda-trójkąt}

\subsubsection{Trójkąt}
\begin{schemat}
\draw
 node[ocirc] (A) at (   0, 3.5  ) {$A$}
 node[ocirc] (B) at (-3.5,-2.5  ) {$B$}
 node[ocirc] (C) at ( 3.5,-2.5  ) {$C$}
 
 node[circ] (Aa) at ( 0, 2) {}
 node[circ] (Bb) at (-2, -1.5) {}
 node[circ] (Cc) at ( 2, -1.5) {}
 
 (A) to[short] (Aa)
 (B) to[short] (Bb)
 (C) to[short] (Cc)
 
 (Aa) to[R,l=$R_1$] (Bb)
 (Aa) to[R,l=$R_2$] (Cc)
 (Bb) to[R,l=$R_3$] (Cc) 
;
\end{schemat}

\subsubsection{Gwiazda}
\begin{schemat}
\draw
 node[ocirc] (A) at (   0, 3.5  ) {$A$}
 node[ocirc] (B) at (-3.5,-2.5  ) {$B$}
 node[ocirc] (C) at ( 3.5,-2.5  ) {$C$}
 node[circ ] (D) at (   0,-0.5  ) {   }
 (A) to[R,l=$R_A$] (D)
 (B) to[R,l=$R_B$] (D)
 (C) to[R,l=$R_C$] (D) 
;
\end{schemat}

\subsubsection{Przekształcenie trójkat-gwiazda}
\begin{equation}
R_A=\frac{R_1 \cdot R_2}{R_1 + R_2 + R_3}
\end{equation}
\begin{equation}
R_B=\frac{R_1 \cdot R_3}{R_1 + R_2 + R_3}
\end{equation}
\begin{equation}
R_C=\frac{R_2 \cdot R_3}{R_1 + R_2 + R_3}
\end{equation}

\subsubsection{Przekształcenie gwiazda-trójkąt}
\begin{equation}
R_1=R_A+R_B+\frac{R_A \cdot R_B}{R_C}
\end{equation}
\begin{equation}
R_2=R_A+R_C+\frac{R_A \cdot R_C}{R_B}
\end{equation}
\begin{equation}
R_3=R_b+R_C+\frac{R_B \cdot R_C}{R_A}
\end{equation}